generator/characteristic.ml
@@ -1420,6 +1420,7 @@ and cfg_algebraics decls =
       let get_typed_constructor (c,ts) =
          check_constr_name loc c;
          (c, coq_impls (List.map (lift_typ_exp loc) ts) ret_typ) in
+      (* ------ inductive definition -------*)
       let coqind_decl =
          if List.length decls = 1 then
             {  coqind_name = type_constr_name x;
@@ -1437,12 +1438,14 @@ and cfg_algebraics decls =
                              (c, coq_foralls (coq_types params) t)
                      ) branches; }
           in
+      (* ------ implicit arguments -------*)
       let implicit_decl =
          match params with
          | [] -> []
          | _ -> List.map (fun (cname,_) -> Coqtop_implicit (cname, List.map (fun p -> p,Coqi_maximal) params)) branches
          in
-      let build_polyeq_axioms (c,ts) =
+      (* ------ polymorphic comparison -------*)
+      let build_polyeq_axioms (c,ts) =  (* LATER: add encoder constraints *)
         let axiom_name = polymorphic_eq_arg_name c in
         let axiom_type =
           let pred = coq_cfml_var "WPBuiltin.polymorphic_eq_arg" in
@@ -1464,7 +1467,92 @@ and cfg_algebraics decls =
             Hint Resolve polymorphic_eq_arg_some : polymorphic_eq.
           *)
       let polyeq_axioms = List.map build_polyeq_axioms branches in
-      (coqind_decl, (implicit_decl @ List.concat polyeq_axioms))
+      (* ------ encoders -------*)
+      (* Example: see SepLifted.v section EncList *)
+
+      let context_vars = Formula.enc_args params in
+
+      let impl_name = encoder_impl x in
+      let inj_name = encoder_injective x in
+      let inst_name = encoder_instance x in
+      let rec_name = "f__" in
+      let arg_name = "v__" in
+      let patvar_name i = "x" ^ (string_of_int i) ^ "__" in
+
+      let impl_branch (c,ts) =
+         let n = List.length ts in
+         let enc_arg i t =
+            let arg = coq_var (patvar_name i) in
+            let is_recursive_call =
+              let c0, cs = coq_apps_inv t in
+              match c0 with
+              | Coq_var c2 -> (c = c2) (* LATER: check full paths *)
+              | _ -> failwith "unrecognized type for a constructor argument"
+              in
+            let encoder =
+              if is_recursive_call
+                then coq_var rec_name
+                else enc (* the typeclass encoder *)
+              in
+            coq_app encoder arg
+            in
+         let pat = coq_apps (coq_var c) (list_init n (fun i -> coq_var (patvar_name i))) in
+         let res = coq_apps val_constr [(coq_string_val c); (coq_list ~typ:val_type (List.mapi enc_arg ts))] in
+         (pat, res) in
+
+      let impl_body = coq_match (coq_var arg_name) (List.map impl_branch branches) in
+      let impl_func = coq_fixs rec_name [(arg_name, ret_typ)] coq_val impl_body in
+      let encoder_def = Coqtop_def ((impl_name, Coq_wild), impl_func) in
+
+      let injectivity_axiom = Coqtop_param (inj_name, coq_app coq_injective impl_name) in
+
+      let instance_impl = coq_app enc_make inj_name in
+      let encoder_instance = Coqtop_instance ((inst_name, enc_type ret_typ), instance_impl, true) in
+
+      let section_items = [ encoder_def; injectivity_axiom; encoder_instance ] in
+      let encoders_defs = coqtops_section_context (encoder_section x) context_vars section_items in
+
+
+(*
+and encoder_algebraic d =
+  let tname = name_type d.atypalg_name in
+  let make_args x =
+    let tname_arg = name_type x in
+    [ (tname_arg, Cexp_var "Set");
+      (name_encoder tname_arg, Cexp_apply (Cexp_var name_code, [Cexp_var tname_arg])) ] in
+  let branch (c,ts) =
+     let nb = List.length ts in
+     let vars = name_arg_list nb in
+     let pat = Cpat_constr (c, List.map (fun xi -> Cpat_var xi) vars) in
+     let make_item x t =
+       Cexp_apply (encoder_type t, [Cexp_var x]) in
+     let con_args = Cexp_list (List.map2 make_item vars ts) in
+     let body = Cexp_apply (Cexp_var name_val_con,
+                            [ Cexp_var (name_constr c); con_args ] ) in
+     (pat, body) in
+  let last_arg_type = Cexp_apply (Cexp_var tname, List.map (fun x -> Cexp_var (name_type x)) d.atypalg_params) in
+  let last_arg = (name_encoded, last_arg_type) in
+  { cfixdef_name = name_encoder tname;
+    cfixdef_args = (List.concat (List.map make_args d.atypalg_params)) @ [ last_arg ];
+    cfixdef_ret = Cexp_var name_val; ----Cexp_apply (Cexp_var name_code, [Cexp_var tname]);
+    cfixdef_decr = name_encoded;
+    cfixdef_body = Cexp_match (Cexp_var name_encoded, List.map branch d.atypalg_cases);
+  }
+
+and encoder_type = function
+   | Atyp_var x -> Cexp_var (name_encoder x)
+   | Atyp_arrow (t1,t2) -> Cexp_var (name_encoder name_val)
+   | Atyp_tuple [] -> assert false
+   | Atyp_tuple ts -> Cexp_apply (Cexp_var (name_encoder (name_tuple (List.length ts))),
+                                  List.map encoder_type ts)
+   | Atyp_constr (id, ts) -> Cexp_apply (Cexp_var (name_encoder (lident_to_str id)),
+                                         List.map encoder_type ts)
+
+*)
+
+
+      (* ------ everything-------*)
+      (coqind_decl, (implicit_decl @ List.concat polyeq_axioms) @ encoders_defs)
       in
    let inds,tops = List.split (List.map trans_ind decls) in
      [ Coqtop_ind inds ]
