lib/stdlib/go.sh
@@ -1,0 +1,4 @@
+source ~/conf/bashcode.sh
+make -f Makefile.dev _CoqProject
+make -f Makefile.dev vo
+# dev vo
